updated to use new homotopy definition

src/homotopy_test.lean
@@ -1,64 +1,56 @@
 import algebraic_topology.simplicial_set
 import combinatorics.quiver.path
-import simplicial_paths
+import path_homotopy
 
 open quiver
 
-variable X : sSet
+variable {X : sSet}
 
-infix `**`:50 := path.comp
-
--- witnesses 0-simplices a, b as the boundary of 1-simplex ab
-def ends (ab : X _[1]) (a b : X _[0]) := (X.δ 1 ab = a) ∧ (X.δ 0 ab = b)
--- produces a path a -> b given a proof that a, b are the boundary of a 1-simplex
-def to_path {ab : X _[1]} {a b : X _[0]} (ε : ends X ab a b) :=
-  edge_to_path ab a b ε.1 ε.2
 
 -- triangle witnessing composition A -> B -> C = A -> C
 lemma triangle (a b c : X _[0]) (ab bc ac : X _[1]) (abc : X _[2])
-    {εab : ends X ab a b}  {εbc : ends X bc b c} {εac : ends X ac a c}
+    {εab : ends ab a b}  {εbc : ends bc b c} {εac : ends ac a c}
     {d0 : X.δ 0 abc = bc} {d1 : X.δ 1 abc = ac} {d2 : X.δ 2 abc = ab} :
 
-    homotopic a c (to_path X εac) ((to_path X εab) ** (to_path X εbc)) :=
+    homotopic a c (to_path εac) ((to_path εab) ** (to_path εbc)) :=
 begin
-    apply homotopic.lift, apply homotopic'.lift,
+    apply homotopic.lift,
     subst d0, subst d1, subst d2,
     apply homotopic''.homotopy,
 end
 
 -- commutative square witnessing A -> B -> C = A -> D -> C = A -> C
 lemma comm_square (a b c d : X _[0]) (ab bc ad dc ac : X _[1]) (abc adc : X _[2])
-    {εab : ends X ab a b} {εbc : ends X bc b c} {εad : ends X ad a d}
-    {εdc : ends X dc d c} {εac : ends X ac a c}
+    {εab : ends ab a b} {εbc : ends bc b c} {εad : ends ad a d}
+    {εdc : ends dc d c} {εac : ends ac a c}
     {_ : X.δ 0 abc = bc} {_ : X.δ 1 abc = ac} {_ : X.δ 2 abc = ab}
     {_ : X.δ 0 adc = dc} {_ : X.δ 1 adc = ac} {_ : X.δ 2 adc = ad} :
 
-    homotopic a c ((to_path X εab) ** (to_path X εbc)) ((to_path X εad) ** (to_path X εdc)) :=
+    homotopic a c ((to_path εab) ** (to_path εbc)) ((to_path εad) ** (to_path εdc)) :=
 begin
-    apply homotopic.lift,
-    apply homotopic'.trans, apply homotopic.lift, apply homotopic'.symm, 
-    refine triangle X a b c ab bc ac abc; assumption,
-    refine triangle X a d c ad dc ac adc; assumption,
+    apply homotopic.trans, apply homotopic.symm, 
+    refine triangle a b c ab bc ac abc; assumption,
+    refine triangle a d c ad dc ac adc; assumption,
 end
 
 
 lemma two_triangles (a b c d e : X _[0]) (ab bc ac cd de ce : X _[1]) (abc cde : X _[2])
-    {εab : ends X ab a b} {εbc : ends X bc b c} {εac : ends X ac a c}
-    {εcd : ends X cd c d} {εde : ends X de d e} {εce : ends X ce c e}
+    {εab : ends ab a b} {εbc : ends bc b c} {εac : ends ac a c}
+    {εcd : ends cd c d} {εde : ends de d e} {εce : ends ce c e}
 
     {_ : X.δ 0 abc = bc} {_ : X.δ 1 abc = ac} {_ : X.δ 2 abc = ab}
     {_ : X.δ 0 cde = de} {_ : X.δ 1 cde = ce} {_ : X.δ 2 cde = cd} :
 
-    homotopic a e ((to_path X εac) ** (to_path X εce)) ((to_path X εab) ** (to_path X εbc) ** (to_path X εcd) ** (to_path X εde)) :=
+    homotopic a e ((to_path εac) ** (to_path εce)) ((to_path εab) ** (to_path εbc) ** (to_path εcd) ** (to_path εde)) :=
 begin
-  have H1 : homotopic a e ((to_path X εac) ** (to_path X εce)) ((to_path X εab) ** (to_path X εbc) ** (to_path X εce)),
+  have H1 : homotopic a e ((to_path εac) ** (to_path εce)) ((to_path εab) ** (to_path εbc) ** (to_path εce)),
   apply homotopic.comp_r,
-  refine triangle X a b c ab bc ac abc; assumption,
+  refine triangle a b c ab bc ac abc; assumption,
   
-  have H2 : homotopic a e ((to_path X εab) ** (to_path X εbc) ** (to_path X εce)) ((to_path X εab) ** (to_path X εbc) ** (to_path X εcd) ** (to_path X εde)),
-  rw path.comp_assoc (to_path X εab**to_path X εbc),
+  have H2 : homotopic a e ((to_path εab) ** (to_path εbc) ** (to_path εce)) ((to_path εab) ** (to_path εbc) ** (to_path εcd) ** (to_path εde)),
+  rw path.comp_assoc (to_path εab**to_path εbc),
   apply homotopic.comp_l,
-  refine triangle X c d e cd de ce cde; assumption,
+  refine triangle c d e cd de ce cde; assumption,
   
-  apply homotopic.lift, apply homotopic'.trans, refine H1, refine H2,
+  apply homotopic.trans, refine H1, refine H2,
 end
